Characterizer basically done for Id monad

MonadicHHL/Characterizer.lean
@@ -1,21 +1,15 @@
 import MonadicHHL.HHLMonads
 
+--- Characterizer definition
+
 -- For the simplest case : Set α → Set β
 structure charact_path (α β : Type _) where
   pc : α → Prop -- or Bool?
   res : α → β
 
-def id_charact_path {α : Type _} : charact_path α α :=
-  { pc := fun _ => true,
-    res := fun y => y }
-
 abbrev characterizer (α β : Type _) : Type := List (charact_path α β)
 
-def characterizer_pure {α β : Type _} (x : β) : characterizer α β :=
-  [ {
-      pc := fun _ => true,
-      res := fun _ => x
-  } ]
+--- Characterizer soundness
 
 def characterizer_sound {α β : Type _}
   (C : α → Id β) (charac : characterizer α β) : Prop :=
@@ -46,6 +40,44 @@ lemma characterizer_sound_altE {α β : Type _}
     specialize h cp
     aesop
 
+lemma characterizer_sound_set_view {α β : Type _}
+  {C : α → Id β} {charac : characterizer α β}
+  (h : characterizer_sound C charac)
+  (S : Set α) :
+  C '' S = { σ' | ∃σ ∈ S, ∃ cp ∈ charac, cp.pc σ ∧ cp.res σ = σ' }
+  := by
+    apply Set.ext
+    intro σ'
+    simp [Set.image]
+    apply Iff.intro
+    {
+      intro h
+      rcases h with ⟨σ, inS, hC⟩
+      have hcp := characterizer_soundE h σ
+      rcases hcp with ⟨cp, cp_in, cp_pc, cp_res⟩
+      apply Exists.intro σ
+      simp [inS]
+      apply Exists.intro cp
+      simp [cp_in, cp_pc, cp_res, hC]
+    }
+    {
+      intro h
+      rcases h with ⟨σ, inS, ⟨cp, cp_in, cp_pc, cp_res⟩⟩
+      have hC := characterizer_sound_altE h cp σ (cp.res σ)
+      apply Exists.intro σ
+      simp [inS]
+      aesop
+    }
+
+
+------ Sound characterizers for pure, bind, if ------
+
+def characterizer_pure {α β : Type _} (x : β) : characterizer α β :=
+  [ {
+      pc := fun _ => true,
+      res := fun _ => x
+  } ]
+
 lemma characterizer_sound_id {α β : Type _} (x : β) :
   characterizer_sound (fun (_ : α) => pure x) (characterizer_pure x) := by
   simp [characterizer_sound, characterizer_pure]
@@ -63,7 +95,7 @@ def bind_characterizers {α β γ : Type _}
   (charac2 : characterizer β γ) : characterizer α γ :=
   List.map combine_characts (List.product charac1 charac2)
 
-lemma bind_characterizers_sound_simplified {α β γ : Type _}
+lemma bind_characterizers_sound {α β γ : Type _}
   {C1 : α → Id β} {C2 : β → Id γ}
   {charac1 : characterizer α β}
   {charac2 : characterizer β γ}
@@ -133,3 +165,419 @@ lemma concat_for_branch {α β : Type _}
       aesop
     }
   }
+
+
+def generic_characterizer {α β : Type _}
+  (C : α → Id β) : characterizer α β :=
+  [{
+    pc := fun _ => true,
+    res := C
+  }]
+
+lemma generic_characterizer_sound {α β : Type _}
+  (C : α → Id β) :
+  characterizer_sound C (generic_characterizer C) := by
+  simp [characterizer_sound, generic_characterizer]
+  aesop
+
+--------- WP from characterizers ------
+
+def hyperassertion (α : Type _) := Set α → Prop
+
+def triple {α β : Type _}
+  (P : hyperassertion α) (C : α → Id β) (Q : hyperassertion β) : Prop :=
+  ∀ S, P S → Q (C '' S)
+
+def is_WP {α β : Type _}
+  (C : α → Id β) (Q : hyperassertion β) (P : hyperassertion α) : Prop :=
+  triple P C Q ∧
+  (∀ P', triple P' C Q → (∀ S, P' S → P S))
+
+lemma is_WP_unique {α β : Type _}
+  (C : α → Id β) (Q : hyperassertion β)
+  (P1 P2 : hyperassertion α)
+  (h1 : is_WP C Q P1)
+  (h2 : is_WP C Q P2) :
+  P1 = P2 :=
+  by
+    apply Set.ext
+    intro S
+    simp [is_WP] at h1 h2
+    aesop
+
+lemma is_WP_obvious {α β : Type _}
+  (C : α → Id β) (Q : hyperassertion β) :
+  is_WP C Q (fun S => Q (C '' S))
+  := by simp [is_WP, triple]
+
+lemma is_WPE {α β : Type _}
+  {P : hyperassertion α}
+  {C : α → Id β}
+  {Q : hyperassertion β}
+  (h : is_WP C Q P)
+: (∀ S, P S = Q (C '' S))
+:= by
+  have heq : P = (fun S => Q (C '' S)) := by
+    apply is_WP_unique C Q _ _ h
+    apply is_WP_obvious
+  aesop
+
+/-
+def WP_forall_from_charact {α β : Type _}
+  (charac : characterizer α β) (Q : β → Prop) : hyperassertion α :=
+  fun S => ∀σ ∈ S, ∀ cp ∈ charac, cp.pc σ → Q (cp.res σ)
+
+lemma WP_forall_from_charact_is_WP {α β : Type _} {C : α → Id β} {charac : characterizer α β}
+  (h : characterizer_sound C charac)
+  (Q : β → Prop) :
+  is_WP C (fun S => ∀σ ∈ S, Q σ) (WP_forall_from_charact charac Q) :=
+  by
+    constructor
+    {
+      intro S hP
+      simp [WP_forall_from_charact] at hP
+      simp [Set.image]
+      intro a ha
+      have hcp := characterizer_soundE h a
+      rcases hcp with ⟨cp, cp_in, cp_pc, cp_res⟩
+      specialize hP a ha cp cp_in cp_pc
+      aesop
+    }
+    {
+      intro P' htriple S hP
+      simp [WP_forall_from_charact]
+      intro σ hσ cp cp_in cp_pc
+      have hcp := characterizer_sound_altE h cp σ (cp.res σ)
+      aesop
+    }
+
+def WP_exists_from_charact {α β : Type _}
+  (charac : characterizer α β) (Q : β → Prop) : hyperassertion α :=
+  fun S => ∃σ ∈ S, ∃ cp ∈ charac, cp.pc σ ∧ Q (cp.res σ)
+
+lemma WP_exists_from_charact_is_WP {α β : Type _} {C : α → Id β} {charac : characterizer α β}
+  (h : characterizer_sound C charac)
+  (Q : β → Prop) :
+  is_WP C (fun S => ∃σ ∈ S, Q σ) (WP_exists_from_charact charac Q) :=
+  by
+    constructor
+    {
+      intro S hP
+      simp [WP_exists_from_charact] at hP
+      simp [Set.image]
+      rcases hP with ⟨σ, inS, ⟨cp, hcp⟩⟩
+      apply Exists.intro σ
+      simp [inS]
+      have hcp' := characterizer_sound_altE h cp σ (cp.res σ)
+      aesop
+    }
+    {
+      intro P' htriple S hP
+      simp [WP_exists_from_charact]
+      simp [triple] at htriple
+      specialize htriple S hP
+      rcases htriple with ⟨σ, inS, hh⟩
+      apply Exists.intro σ
+      simp [inS]
+      have hcp := characterizer_soundE h σ
+      aesop
+    }
+-/
+
+--- "Constructors"
+
+def H.pure {α : Type _} (P : Prop) : hyperassertion α :=
+  fun _ => P
+
+def H.forall {α : Type _} (P : α → hyperassertion α) : hyperassertion α :=
+  fun S => ∀ σ ∈ S, P σ S
+
+def H.exists {α : Type _} (P : α → hyperassertion α) : hyperassertion α :=
+  fun S => ∃ σ ∈ S, P σ S
+
+---- Example
+
+abbrev forall_forall_post {β : Type _} (Q : β → β → Prop) : hyperassertion β :=
+  H.forall (fun σ1 => H.forall (fun σ2 => H.pure (Q σ1 σ2)))
+
+def WP.forall {α β : Type _}
+  (charac : characterizer α β) (P : β → hyperassertion α) : hyperassertion α :=
+  fun S =>
+    ∀ σ ∈ S, ∀ cp ∈ charac, cp.pc σ → P (cp.res σ) S
+
+def WP.exists {α β : Type _}
+  (charac : characterizer α β) (P : β → hyperassertion α) : hyperassertion α :=
+  fun S =>
+    ∃ σ ∈ S, ∃ cp ∈ charac, cp.pc σ ∧ P (cp.res σ) S
+
+lemma triple_cons_post {α β : Type _}
+  (P : hyperassertion α)
+  (C : α → Id β)
+  (Q Q' : hyperassertion β)
+  (htriple : triple P C Q')
+  (hcons : ∀ S, Q' S → Q S)
+  : triple P C Q :=
+  by
+    simp [triple] at *
+    aesop
+
+@[grind .]
+lemma is_WP_forall_comp {α β : Type _} {C : α → Id β} {charac : characterizer α β}
+  (h : characterizer_sound C charac)
+  (Q : β → hyperassertion β)
+  (P : β → hyperassertion α)
+  (hh : ∀ σ', is_WP C (Q σ') (P σ')) :
+  is_WP C (H.forall Q) (WP.forall charac P) := by
+    have heq : WP.forall charac P = (fun S => H.forall Q (C '' S)) := by
+    {
+      apply funext
+      intro S
+      simp [WP.forall, H.forall]
+      have hsimpler : ∀ σ ∈ S, (∀ cp ∈ charac, cp.pc σ → P (cp.res σ) S) ↔ (Q (C σ) (C '' S)) := by
+      {
+        intro σ hS
+        apply Iff.intro
+        {
+          intro hcp
+          have hh := is_WPE (hh (C σ)) S
+          rw [hh.symm]
+          have h := characterizer_soundE h σ
+          rcases h with ⟨cp, cp_in, cp_pc, cp_res⟩
+          specialize hcp cp cp_in cp_pc
+          aesop
+        }
+        {
+          intro hQ cp cp_in cp_pc
+          have hh := is_WPE (hh (C σ)) S
+          have hcp := characterizer_sound_altE h cp σ (cp.res σ)
+          aesop
+        }
+      }
+      aesop
+    }
+    rw [heq]
+    apply is_WP_obvious
+
+@[grind .]
+lemma is_WP_exists_comp {α β : Type _} {C : α → Id β} {charac : characterizer α β}
+  (h : characterizer_sound C charac)
+  (Q : β → hyperassertion β)
+  (P : β → hyperassertion α)
+  (hh : ∀ σ', is_WP C (Q σ') (P σ')) :
+  is_WP C (H.exists Q) (WP.exists charac P) := by
+    have heq : WP.exists charac P = (fun S => H.exists Q (C '' S)) := by
+    {
+      apply funext
+      intro S
+      simp [WP.exists, H.exists]
+      have hsimpler : ∀ σ ∈ S, (∃ cp ∈ charac, cp.pc σ ∧ P (cp.res σ) S) ↔ (Q (C σ) (C '' S)) := by
+        {
+          intro σ hS
+          apply Iff.intro
+          {
+            intro hcp
+            rcases hcp with ⟨cp, cp_in, cp_pc, cp_res⟩
+            have hh := is_WPE (hh (C σ)) S
+            have h := characterizer_sound_altE h cp σ
+            aesop
+          }
+          {
+            intro hQ
+            have hcp := characterizer_soundE h σ
+            have hh := is_WPE (hh (C σ)) S
+            aesop
+          }
+        }
+      grind
+    }
+    rw [heq]
+    apply is_WP_obvious
+
+
+@[simp, grind .]
+lemma is_WP_pure {α β : Type _} {C : α → Id β} (P : Prop)
+  : is_WP C (H.pure P) (H.pure P)
+  := by simp [is_WP, triple, H.pure]
+
+lemma elim_triple {α β : Type _}
+  {P : hyperassertion α}
+  {C : α → Id β}
+  {Q : hyperassertion β}
+  (htriple : triple P C Q)
+  (S : Set α)
+  (hP : P S) :
+  Q (C '' S) :=
+  by
+    simp [triple] at htriple
+    specialize htriple S hP
+    aesop
+
+@[grind .]
+lemma is_WP_and {α β : Type _} {C : α → Id β}
+  {P1 P2 : hyperassertion α}
+  {Q1 Q2 : hyperassertion β}
+  (h1 : is_WP C Q1 P1)
+  (h2 : is_WP C Q2 P2) :
+  is_WP C (fun S => Q1 S ∧ Q2 S) (fun S => P1 S ∧ P2 S) :=
+  by
+    have h1 := is_WPE h1
+    have h2 := is_WPE h2
+    simp [is_WP, triple]
+    aesop
+
+@[grind .]
+lemma is_WP_or {α β : Type _} {C : α → Id β}
+  {P1 P2 : hyperassertion α}
+  {Q1 Q2 : hyperassertion β}
+  (h1 : is_WP C Q1 P1)
+  (h2 : is_WP C Q2 P2) :
+  is_WP C (fun S => Q1 S ∨ Q2 S) (fun S => P1 S ∨ P2 S) :=
+  by
+    have h1 := is_WPE h1
+    have h2 := is_WPE h2
+    simp [is_WP, triple]
+    aesop
+
+lemma is_WP_forall_normal {α β γ : Type _} {C : α → Id β}
+  (Q : γ → hyperassertion β)
+  (P : γ → hyperassertion α)
+  (hh : ∀ x, is_WP C (Q x) (P x)) :
+  is_WP C (fun S => ∀ x, Q x S) (fun S => ∀ x, P x S) := by
+    constructor
+    {
+      intro S h x
+      have hh := is_WPE (hh x) S
+      aesop
+    }
+    {
+      intro P' htriple S hP x
+      have hh := is_WPE (hh x) S
+      aesop
+    }
+
+lemma is_WP_exists_normal {α β γ : Type _} {C : α → Id β}
+  (Q : γ → hyperassertion β)
+  (P : γ → hyperassertion α)
+  (hh : ∀ x, is_WP C (Q x) (P x)) :
+  is_WP C (fun S => ∃ x, Q x S) (fun S => ∃ x, P x S) := by
+    constructor
+    {
+      simp [triple]
+      intro S x
+      have hh := is_WPE (hh x)
+      aesop
+    }
+    {
+      intro P' htriple S hP
+      have htriple := elim_triple htriple S hP
+      rcases htriple with ⟨x, h'⟩
+      have hh := is_WPE (hh x) S
+      aesop
+    }
+
+
+
+
+
+
+--------------------------
+-- Examples
+--------------------------
+
+-- Forall
+
+example {α β : Type _} {C : α → Id β} {charac : characterizer α β}
+  (h : characterizer_sound C charac) (Q : β → Prop) :
+  is_WP C
+    (H.forall (fun σ => H.pure (Q σ)))
+    (WP.forall charac (fun σ => H.pure (Q σ)))
+  := by grind
+
+example {α β : Type _} {C : α → Id β} {charac : characterizer α β}
+  (h : characterizer_sound C charac) (Q : β → β → Prop) :
+  is_WP C
+    (H.forall (fun σ1 => H.forall (fun σ2 => H.pure (Q σ1 σ2))))
+    (WP.forall charac (fun σ1 => WP.forall charac (fun σ2 => H.pure (Q σ1 σ2))))
+  := by grind
+
+-- Exists
+
+example {α β : Type _} {C : α → Id β} {charac : characterizer α β}
+  (h : characterizer_sound C charac) (Q : β → Prop) :
+  is_WP C
+    (H.exists (fun σ => H.pure (Q σ)))
+    (WP.exists charac (fun σ => H.pure (Q σ)))
+  := by grind
+
+example {α β : Type _} {C : α → Id β} {charac : characterizer α β}
+  (h : characterizer_sound C charac) (Q : β → β → Prop) :
+  is_WP C
+    (H.exists (fun σ1 => H.exists (fun σ2 => H.pure (Q σ1 σ2))))
+    (WP.exists charac (fun σ1 => WP.exists charac (fun σ2 => H.pure (Q σ1 σ2))))
+  := by grind
+
+-- Mixed
+
+example {α β : Type _} {C : α → Id β} {charac : characterizer α β}
+  (h : characterizer_sound C charac) (Q : β → β → Prop) :
+  is_WP C
+    (H.forall (fun σ1 => H.exists (fun σ2 => H.pure (Q σ1 σ2))))
+    (WP.forall charac (fun σ1 => WP.exists charac (fun σ2 => H.pure (Q σ1 σ2))))
+  := by grind
+
+example {α β : Type _} {C : α → Id β} {charac : characterizer α β}
+  (h : characterizer_sound C charac) (Q : β → β → Prop) :
+  is_WP C
+    (H.exists (fun σ1 => H.forall (fun σ2 => H.pure (Q σ1 σ2))))
+    (WP.exists charac (fun σ1 => WP.forall charac (fun σ2 => H.pure (Q σ1 σ2))))
+  := by grind
+
+
+/-
+
+def WP_forall_forall_from_charact {α β : Type _}
+  (charac : characterizer α β) (Q : β → β → Prop) : hyperassertion α :=
+  fun S =>
+    ∀ a1 ∈ S, ∀cp1 ∈ charac, cp1.pc a1 →
+    ∀ a2 ∈ S, ∀cp2 ∈ charac, cp2.pc a2 →
+      Q (cp1.res a1) (cp2.res a2)
+
+lemma same_hyperassertions {β : Type _} (Q : β → β → Prop) :
+  (fun S => ∀σ1 ∈ S, ∀σ2 ∈ S, Q σ1 σ2) = forall_forall_post Q
+  := rfl
+
+lemma WP_forall_forall_from_charact_sound {α β : Type _} {C : α → Id β} {charac : characterizer α β}
+  (h : characterizer_sound C charac)
+  (Q : β → β → Prop) :
+  is_WP C
+    -- (forall_forall_post Q)
+    (fun S => ∀σ1 ∈ S, ∀σ2 ∈ S, Q σ1 σ2)
+    (WP_forall_forall_from_charact charac Q) :=
+  by
+    constructor
+    {
+      simp [triple, WP_forall_forall_from_charact, Set.image]
+      intro S hP σ1 h1 σ2 h2
+      have hcp1 := characterizer_soundE h σ1
+      rcases hcp1 with ⟨cp1, cp1_in, cp1_pc, cp1_res⟩
+      have hcp2 := characterizer_soundE h σ2
+      rcases hcp2 with ⟨cp2, cp2_in, cp2_pc, cp2_res⟩
+      specialize hP σ1 h1 cp1 cp1_in cp1_pc σ2 h2 cp2 cp2_in cp2_pc
+      aesop
+    }
+    {
+      intro P' htriple S hP
+      simp [WP_forall_forall_from_charact]
+      intro σ1 h1 cp1 cp1_in cp1_pc σ2 h2 cp2 cp2_in cp2_pc
+      have hcp1 := characterizer_sound_altE h cp1 σ1 (cp1.res σ1)
+      have hcp2 := characterizer_sound_altE h cp2 σ2 (cp2.res σ2)
+      specialize htriple S hP
+      aesop
+    }
+
+lemma WP_forall_forall_same {α β : Type _}
+  (charac : characterizer α β) (Q : β → β → Prop) :
+  WP_forall_forall_from_charact charac Q = WP_forall_forall_from_charact_comp charac Q
+  := rfl
+
+-/
